fixed expression evaluation function

BoogieLang/RedExprFunction.thy
@@ -2,58 +2,42 @@ theory RedExprFunction
 imports Semantics
 begin
 
-fun expr_size :: "expr \<Rightarrow> nat"
-  where
-    "expr_size (Var x) = 0"
-  | "expr_size (Val v) = 0"
-  | "expr_size (BVar v) = 0"
-  | "expr_size (UnOp up e) = size(e)+1"
-  | "expr_size (e1 \<guillemotleft>bop\<guillemotright> e2) = size(e1)+size(e2)+1"
-  | "expr_size (FunExp f args) = (sum_list (map size args))+1"
-  | "expr_size (Forall ty e) = size(e)+1"
-  | "expr_size (Exists ty e) = size(e)+1"
-
-lemma map_eq: "\<lbrakk>\<forall>i. (f (xs ! i) = f (ys ! i)); length xs = length ys\<rbrakk> \<Longrightarrow> map f xs = map f ys"
-  sorry
-
-lemma size_eopen: "size (eopen i (Val v) e) = size e"
-proof (induction e arbitrary: i; (fastforce | tactic \<open>all_tac\<close>))
-case (FunExp f args)
-  have "size (eopen i (Val v) (FunExp f args)) = size (FunExp f (map (eopen i (Val v)) args))" by simp
-  have "map size args = (map size (map (eopen i (Val v)) args))" 
-    apply (rule map_eq)
-     apply rule
-    using FunExp.IH 
-    sorry
-  show ?case sorry
-qed
-
-(* note that BVar x will never need to be evaluated if the expression reduces *)
-function red_expr_fun :: "fun_context \<Rightarrow> expr \<Rightarrow> nstate \<Rightarrow> val"
+fun red_expr_fun :: "'a absval_ty_fun \<Rightarrow> 'a fun_context \<Rightarrow> rtype_env \<Rightarrow> expr \<Rightarrow> 'a nstate \<Rightarrow> 'a val"
   where 
-    "red_expr_fun \<Gamma> (Var x) n_s = the (n_s(x))"
-  | "red_expr_fun \<Gamma> (BVar x) n_s = BoolV False"
-  | "red_expr_fun \<Gamma> (Val v) n_s = v"
-  | "red_expr_fun \<Gamma> (UnOp uop e) n_s = the (unop_eval uop (red_expr_fun \<Gamma> e n_s))"
-  | "red_expr_fun \<Gamma> (e1 \<guillemotleft>bop\<guillemotright> e2) n_s = the (binop_eval bop (red_expr_fun \<Gamma> e1 n_s) (red_expr_fun \<Gamma> e2 n_s))"
-  | "red_expr_fun \<Gamma> (FunExp f args) n_s = 
+    "red_expr_fun A \<Gamma> \<Omega> (Var x) n_s = the (n_s(x))"
+  | "red_expr_fun A \<Gamma> \<Omega> (Lit lit) n_s = LitV lit"
+  | "red_expr_fun A \<Gamma> \<Omega> (UnOp uop e) n_s = the (unop_eval_val uop (red_expr_fun A \<Gamma> \<Omega> e n_s))"
+  | "red_expr_fun A \<Gamma> \<Omega> (e1 \<guillemotleft>bop\<guillemotright> e2) n_s = the (binop_eval_val bop (red_expr_fun A \<Gamma> \<Omega> e1 n_s) (red_expr_fun A \<Gamma> \<Omega> e2 n_s))"
+  | "red_expr_fun A \<Gamma> \<Omega> (FunExp f tys args) n_s = 
       (let f_interp = the ( (snd \<Gamma>) f) in
-      (let v_args = map (\<lambda>e. red_expr_fun \<Gamma> e n_s) args in
-      the (f_interp v_args)))"
-  | "red_expr_fun \<Gamma> (Forall ty e) n_s = 
-        BoolV (\<forall>v. type_of_val v = ty \<longrightarrow> ((red_expr_fun \<Gamma> (eopen 0 (Val v) e) n_s) = BoolV True))"
-  | "red_expr_fun \<Gamma> (Exists ty e) n_s =
-        BoolV (\<exists>v. type_of_val v = ty \<and> ((red_expr_fun \<Gamma> (eopen 0 (Val v) e) n_s) = BoolV True))"
-  by pat_completeness auto
-termination
-  apply (relation "measure (\<lambda>(\<Gamma>, e, n_s). size(e))")
-  apply (simp_all add: size_eopen)
-  using not_less_eq size_list_estimation apply fastforce
-  done
+      (let v_args = map (\<lambda>e. red_expr_fun A \<Gamma> \<Omega> e n_s) args in
+      the (f_interp (map (instantiate \<Omega>) tys) v_args)))"
+  | "red_expr_fun A \<Gamma> \<Omega> (Forall ty e) n_s = 
+        BoolV (\<forall>v. type_of_val A v = instantiate \<Omega> ty \<longrightarrow> ((red_expr_fun A \<Gamma> \<Omega> e (ext_env n_s v)) = BoolV True))"
+  | "red_expr_fun A \<Gamma> \<Omega> (Exists ty e) n_s =
+        BoolV (\<exists>v. type_of_val A v = instantiate \<Omega> ty \<and> ((red_expr_fun A \<Gamma> \<Omega> e (ext_env n_s v)) = BoolV True))"
+  | "red_expr_fun A \<Gamma> \<Omega> (ForallT e) n_s = BoolV (\<forall>t. closed t \<longrightarrow> ((red_expr_fun A \<Gamma> (t#\<Omega>) e n_s) = BoolV True))"
+  | "red_expr_fun A \<Gamma> \<Omega> (ExistsT e) n_s = BoolV (\<exists>t. closed t \<and> ((red_expr_fun A \<Gamma> (t#\<Omega>) e n_s) = BoolV True))"
 
 lemma red_expr_fun_rel:
-  shows "\<Gamma> \<turnstile> \<langle>e, n_s\<rangle> \<Down> v \<Longrightarrow> red_expr_fun \<Gamma> e n_s = v" and
-       "\<Gamma> \<turnstile> \<langle>es, n_s\<rangle> [\<Down>] vs \<Longrightarrow> map (\<lambda> e. red_expr_fun \<Gamma> e n_s) es = vs"
-  by (induction rule: red_expr_red_exprs.inducts, auto)
+  shows "A,\<Gamma>,\<Omega> \<turnstile> \<langle>e, n_s\<rangle> \<Down> v \<Longrightarrow> red_expr_fun A \<Gamma> \<Omega> e n_s = v" and
+       "A,\<Gamma>,\<Omega> \<turnstile> \<langle>es, n_s\<rangle> [\<Down>] vs \<Longrightarrow> map (\<lambda> e. red_expr_fun A \<Gamma> \<Omega> e n_s) es = vs"
+proof (induction rule: red_expr_red_exprs.inducts)
+  case (RedForAllTrue \<Omega> ty e n_s)
+  thus ?case by fastforce
+next
+  case (RedForAllFalse v \<Omega> ty e n_s)
+  hence "\<not>((\<forall>v. type_of_val A v = instantiate \<Omega> ty \<longrightarrow> ((red_expr_fun A \<Gamma> \<Omega> e (ext_env n_s v)) = BoolV True)))"
+    by (metis lit.inject(1) val.inject(1))
+  thus ?case by simp       
+next
+  case (RedExistsTrue v \<Omega> ty e n_s)
+  hence "(\<exists>v. type_of_val A v = instantiate \<Omega> ty \<and> ((red_expr_fun A \<Gamma> \<Omega> e (ext_env n_s v)) = BoolV True))"
+    by blast  
+  thus ?case by simp    
+next
+  case (RedExistsFalse \<Omega> ty e n_s)
+  thus ?case by fastforce
+qed (auto)
 
 end
